keep working on cache

examples/scache/RWLock.i.dfy
@@ -1,7 +1,9 @@
 include "ArrayPtr.s.dfy"
+include "../../lib/Lang/NativeTypes.s.dfy"
 
 module ReadWriteLockResources {
   import Ptrs
+  import opened NativeTypes
 
   function NThreads() : int { 24 }
 
@@ -21,9 +23,9 @@ module ReadWriteLockResources {
     | Write
     | Back_PendingWrite
 
-  datatype R =
+  datatype Q =
     | FlagsField(ptr: Ptrs.Ptr, flags: Flag)
-    | ReadRefCount(ptr: Ptrs.Ptr, t: int, refcount: int)
+    | ReadRefCount(ptr: Ptrs.Ptr, t: int, refcount: uint8)
 
     | ReadPending(ptr: Ptrs.Ptr, t: int)
     | ReadObtained(ptr: Ptrs.Ptr, t: int)
@@ -34,12 +36,12 @@ module ReadWriteLockResources {
     | WritePending(ptr: Ptrs.Ptr, visited: int)
     | WriteObtained(ptr: Ptrs.Ptr)
 
-  datatype Step =
+  datatype QStep =
     | TakeBackStep(ptr: Ptrs.Ptr)
     | TakeWrite(ptr: Ptrs.Ptr)
     | TakeWriteAwaitBack(ptr: Ptrs.Ptr)
 
-  predicate TakeBack(a: multiset<R>, b: multiset<R>, ptr: Ptrs.Ptr)
+  predicate TakeBack(a: multiset<Q>, b: multiset<Q>, ptr: Ptrs.Ptr)
   {
     && a == multiset{ FlagsField(ptr, Free) }
     && b == multiset{
@@ -48,7 +50,7 @@ module ReadWriteLockResources {
     }
   }
 
-  predicate TakeWrite(a: multiset<R>, b: multiset<R>, ptr: Ptrs.Ptr)
+  predicate TakeWrite(a: multiset<Q>, b: multiset<Q>, ptr: Ptrs.Ptr)
   {
     && a == multiset{ FlagsField(ptr, Free) }
     && b == multiset{
@@ -57,7 +59,7 @@ module ReadWriteLockResources {
     }
   }
 
-  predicate TakeWriteAwaitBack(a: multiset<R>, b: multiset<R>, ptr: Ptrs.Ptr)
+  predicate TakeWriteAwaitBack(a: multiset<Q>, b: multiset<Q>, ptr: Ptrs.Ptr)
   {
     && a == multiset{ FlagsField(ptr, Back) }
     && b == multiset{
@@ -66,7 +68,7 @@ module ReadWriteLockResources {
     }
   }
 
-  predicate TakeWriteFinishBack(a: multiset<R>, b: multiset<R>, ptr: Ptrs.Ptr, fl: Flag)
+  predicate TakeWriteFinishBack(a: multiset<Q>, b: multiset<Q>, ptr: Ptrs.Ptr, fl: Flag)
   {
     // The 'free' case cannot actually occur, but it's convenient to allow it.
     && (fl == Write || fl == Free)
@@ -80,7 +82,7 @@ module ReadWriteLockResources {
     }
   }
 
-  predicate TakeWriteCheckReadZero(a: multiset<R>, b: multiset<R>, ptr: Ptrs.Ptr, idx: int)
+  predicate TakeWriteCheckReadZero(a: multiset<Q>, b: multiset<Q>, ptr: Ptrs.Ptr, idx: int)
   {
     && a == multiset{
       WritePending(ptr, idx),
@@ -92,7 +94,7 @@ module ReadWriteLockResources {
     }
   }
 
-  predicate TakeWriteFinish(a: multiset<R>, b: multiset<R>, ptr: Ptrs.Ptr)
+  predicate TakeWriteFinish(a: multiset<Q>, b: multiset<Q>, ptr: Ptrs.Ptr)
   {
     && a == multiset{
       WritePending(ptr, NThreads())
@@ -102,18 +104,18 @@ module ReadWriteLockResources {
     }
   }
 
-  predicate TakeRead(a: multiset<R>, b: multiset<R>, ptr: Ptrs.Ptr, t: int, r: int)
+  predicate TakeRead(a: multiset<Q>, b: multiset<Q>, ptr: Ptrs.Ptr, t: int, r: uint8)
   {
     && a == multiset{
       ReadRefCount(ptr, t, r)
     }
     && a == multiset{
-      ReadRefCount(ptr, t, r+1),
+      ReadRefCount(ptr, t, if r == 255 then 0 else r+1),
       ReadPending(ptr, t)
     }
   }
 
-  predicate TakeReadFinish(a: multiset<R>, b: multiset<R>, ptr: Ptrs.Ptr, t: int, r: int, fl: Flag)
+  predicate TakeReadFinish(a: multiset<Q>, b: multiset<Q>, ptr: Ptrs.Ptr, t: int, r: uint8, fl: Flag)
   {
     && (fl == Free || fl == Back)
     && a == multiset{
@@ -125,41 +127,48 @@ module ReadWriteLockResources {
     }
   }
 
-  predicate TakeReadBail(a: multiset<R>, b: multiset<R>, ptr: Ptrs.Ptr, t: int, r: int)
+  predicate TakeReadBail(a: multiset<Q>, b: multiset<Q>, ptr: Ptrs.Ptr, t: int, r: uint8)
   {
     && a == multiset{
       ReadRefCount(ptr, t, r),
       ReadPending(ptr, t)
     }
     && b == multiset{
-      ReadRefCount(ptr, t, r-1)
+      ReadRefCount(ptr, t, if r == 0 then 255 else r-1)
     }
   }
 
-  method transform_TakeBack(ptr: Ptrs.Ptr, linear s: R)
-  returns (linear t: R, linear u: R)
+  method transform_TakeBack(ptr: Ptrs.Ptr, linear s: Q)
+  returns (linear t: Q, linear u: Q)
   requires s == FlagsField(ptr, Free)
   ensures t == FlagsField(ptr, Back)
   ensures u == BackObtained(ptr)
 
-  method transform_TakeWrite(ptr: Ptrs.Ptr, linear s: R)
-  returns (linear t: R, linear u: R)
+  method transform_TakeWrite(ptr: Ptrs.Ptr, linear s: Q)
+  returns (linear t: Q, linear u: Q)
   requires s == FlagsField(ptr, Free)
   ensures t == FlagsField(ptr, Write)
   ensures u == WritePendingAwaitBack(ptr)
 
-  method transform_TakeWriteAwaitBack(ptr: Ptrs.Ptr, linear s: R)
-  returns (linear t: R, linear u: R)
+  method transform_TakeWriteAwaitBack(ptr: Ptrs.Ptr, linear s: Q)
+  returns (linear t: Q, linear u: Q)
   requires s == FlagsField(ptr, Back)
   ensures t == FlagsField(ptr, Back_PendingWrite)
   ensures u == WritePendingAwaitBack(ptr)
 
-
-  method transform_TakeWriteFinishBack(ptr: Ptrs.Ptr, fl: Flag, linear s1: R, linear s2: R)
-  returns (linear t1: R, linear t2: R)
+  method transform_TakeWriteFinishBack(ptr: Ptrs.Ptr, fl: Flag, linear s1: Q, linear s2: Q)
+  returns (linear t1: Q, linear t2: Q)
   requires fl == Write || fl == Free
   requires s1 == FlagsField(ptr, fl)
   requires s2 == WritePendingAwaitBack(ptr)
   ensures t1 == FlagsField(ptr, fl)
   ensures t2 == WritePending(ptr, 0)
+
+  method transform_TakeWriteCheckReadZero(ptr: Ptrs.Ptr, idx: int, linear s1: Q, linear s2: Q)
+  returns (linear t1: Q, linear t2: Q)
+  requires s1 == ReadRefCount(ptr, idx, 0)
+  requires s2 == WritePending(ptr, idx)
+  ensures t1 == ReadRefCount(ptr, idx, 0)
+  ensures t2 == WritePending(ptr, idx + 1)
+
 }
