examples/scache/AtomicRefcount.i.dfy
@@ -1,0 +1,62 @@
+include "Atomic.s.dfy"
+include "RWLock.i.dfy"
+include "ArrayPtr.s.dfy"
+include "../../lib/Lang/NativeTypes.s.dfy"
+include "../../lib/Lang/LinearMaybe.s.dfy"
+
+module AtomicRefcount {
+  import opened NativeTypes
+  import opened Ptrs
+  import opened AtomicSpec
+  import ReadWriteLockResources
+
+  type AtomicRefcount = Atomic<uint8, ReadWriteLockResources.Q>
+
+  predicate state_inv(v: uint8, g: ReadWriteLockResources.Q, ptr: Ptr, t: int)
+  {
+    g == ReadWriteLockResources.ReadRefCount(ptr, t, v)
+  }
+
+  predicate atomic_refcount_inv(a: AtomicRefcount, ptr: Ptr, t: int)
+  {
+    forall v, g :: atomic_inv(a, v, g) <==> state_inv(v, g, ptr, t)
+  }
+
+  method unsafe_obtain<R>() returns (linear r: R)
+  method unsafe_dispose<R>(linear r: R)
+
+  method is_refcount_zero(a: AtomicRefcount, ptr: Ptrs.Ptr, t: int,
+      linear m: ReadWriteLockResources.Q)
+  returns (is_zero: bool, linear m': ReadWriteLockResources.Q)
+  requires atomic_refcount_inv(a, ptr, t)
+  requires m == ReadWriteLockResources.WritePending(ptr, t)
+  ensures is_zero ==> m' == ReadWriteLockResources.WritePending(ptr, t + 1)
+  ensures !is_zero ==> m' == ReadWriteLockResources.WritePending(ptr, t)
+  {
+    var c := atomic_read(a);
+
+    ///// Begin jank
+    ///// Setup:
+    var old_v: uint8;
+    var new_v: uint8;
+    linear var old_g: ReadWriteLockResources.Q := unsafe_obtain();
+    assume new_v == old_v;
+    assume c == old_v;
+    assume atomic_inv(a, old_v, old_g);
+    linear var new_g;
+    ///// Transfer:
+    if c == 0 {
+      new_g, m' := ReadWriteLockResources.transform_TakeWriteCheckReadZero(
+          ptr, t, old_g, m);
+    } else {
+      m' := m;
+      new_g := old_g;
+    }
+    ///// Teardown:
+    assert atomic_inv(a, new_v, new_g);
+    unsafe_dispose(new_g);
+    ///// End jank
+
+    is_zero := (c == 0);
+  }
+}
