examples/scache/RWLockResource.i.dfy
@@ -1,0 +1,44 @@
+include "ResourceSpec.s.dfy"
+include "RWLock.i.dfy"
+include "../../lib/Base/Multisets.i.dfy"
+
+module RWLockResource refines ResourceSpec {
+  import opened ReadWriteLockResources
+  import opened Multisets
+
+  datatype R =
+    | LargeFootprint(m: multiset<Q>)
+    | Toe(q: Q)
+
+  predicate Init(s: multiset<R>)
+  {
+    s == multiset{}
+  }
+
+  datatype Step = Step(
+      s: multiset<Q>,
+      s': multiset<Q>,
+      rest: multiset<Q>,
+      qstep: QStep)
+
+  function toe_multiset(s: multiset<Q>) : multiset<R>
+  {
+    Apply((q) => Toe(q), s)
+  }
+
+  predicate transform_step(a: multiset<R>, b: multiset<R>, step: Step)
+  {
+    var lf := LargeFootprint(step.s + step.rest);
+    var lf' := LargeFootprint(step.s' + step.rest);
+    var t := toe_multiset(step.s);
+    var t' := toe_multiset(step.s');
+    && transform_qstep(t, t', step.qstep)
+    && a == multiset{lf} + t
+    && b == multiset{lf'} + t'
+  }
+
+  predicate transform(a: multiset<R>, b: multiset<R>)
+  {
+    exists step :: transform_step(a, b, step)
+  }
+}
